LeanGrow/Src/SampleGenScore/Delab/Test/Term.lean
@@ -1,0 +1,47 @@
+
+
+import LeanGrow.Src.SampleGenScore.Delab.Test.Basic
+import Mathlib.Tactic
+
+
+open Lean
+
+
+theorem tesT_1 (h : n+m = 42) : m+n = 42 :=
+  Nat.add_comm n m ▸ h
+
+#print tesT_1
+
+-- #eval test_apply_sample `tesT_1
+-- #eval test_apply_dig `tesT_1
+-- #eval test_apply_top `tesT_1
+
+
+theorem tesT_2: m+n + 42 = n+m + 42 :=
+  congrArg (· + 42) (Nat.add_comm m n)
+
+#print tesT_2
+
+-- #eval test_apply_sample `tesT_2
+-- #eval test_apply_dig `tesT_2
+-- #eval test_apply_top `tesT_2
+
+
+theorem tesT_3 (x : Int) : (x +1)^2 = 1 + x^2 + 2*x := by ring
+
+#print tesT_3
+
+-- #eval test_apply_sample `tesT_3
+-- #eval test_apply_dig `tesT_3
+-- #eval test_apply_top `tesT_3
+
+
+theorem tesT_4 (x y : Int)  (h1 : x + 1 ≥ 0) (h2 : x = y)
+  : y + 1 ≥ 0 := by
+    grind
+
+#print tesT_4
+
+-- #eval test_apply_sample `tesT_4
+-- #eval test_apply_dig `tesT_4
+-- #eval test_apply_top `tesT_4
