LeanGrow/Src/SampleGenScore/Docs/Preventable.lean
@@ -4,7 +4,7 @@ import Mathlib.Tactic
 
 #check 1
 
--- for linarith, ring & co, find ways to tell from Expr that tactic is applied...
+-- for grind, linarith, ring & co, find ways to tell from Expr that tactic is applied...
 
 open Lean Meta Elab Term Tactic Mathlib
 
@@ -21,5 +21,40 @@ theorem test_2 (x : Int) : (x +1)^2 = 1 + x^2 + 2*x := by ring
 #check Mathlib.Tactic.Linarith.linarith
 
 
+theorem test_1 (x y : Int)  (h1 : x + 1 ≥ 0) (h2 : 5 ≤ y)
+  : x + y + 1 ≥ 5 := by
+    linarith
+
+#print test_1
+
+#check Tactic.Linarith.lt_irrefl
+-- has Mathlib prefix
+
+theorem test_3 (x y : Int)  (h1 : x + 1 ≥ 0) (h2 : 5 ≤ y)
+  : x + y + 1 ≥ 5 := by
+    grind
+
+#print test_3
+#print test_3._proof_1_1
+#check Grind.intro_with_eq
+
+-- Lean prefix
+
+theorem test_4 (x y : Int)  (h1 : x + 1 ≥ 0) (h2 : x = y)
+  : y + 1 ≥ 0 := by
+    grind
+
+#print test_4
+#print test_4._proof_1_1
+
+#check List.perm_append_comm
+
 -- simple rule would be to check if lemma has prefix `Mathlib.Tactic`
 -- since a lot of tactics seem to do this
+
+open List in
+theorem test_5 : ∀ {n : Nat}, length (range' s n step) = n := by grind
+
+#print test_5
+#print test_5._proof_1_1
+-- no grind lemmata
